theories/typing/lib/rwlock/rwlockwriteguard_code.v
@@ -44,7 +44,7 @@ Section rwlockwriteguard_functions.
     iMod ("Hclose" with "[$] HL") as "HL".
     iDestruct (lctx_lft_incl_incl α β with "HL HE") as "#Hαβ"; [solve_typing..|].
     iApply (type_type _ _ _ [ x ◁ box (&shr{α} rwlockwriteguard β ty);
-                              #(shift_loc l' 1) ◁ &shr{α}ty]%TC
+                              #(shift_loc l' 1) ◁ &shr{α}ty]
             with "[] LFT HE Hna HL Hk"); last first.
     { rewrite tctx_interp_cons tctx_interp_singleton tctx_hasty_val tctx_hasty_val' //.
       iFrame. iApply (ty_shr_mono with "[] Hshr'"). iApply lft_incl_glb; first done.
@@ -89,7 +89,7 @@ Section rwlockwriteguard_functions.
     wp_read. iIntros "Hb !>". wp_op. wp_let.
     iMod ("Hcloseα" with "[$H↦]") as "[_ Hα]". iMod ("Hclose" with "Hα HL") as "HL".
     iDestruct (lctx_lft_incl_incl α β with "HL HE") as "#Hαβ"; [solve_typing..|].
-    iApply (type_type _ _ _ [ x ◁ box (uninit 1); #(shift_loc l 1) ◁ &uniq{α}ty]%TC
+    iApply (type_type _ _ _ [ x ◁ box (uninit 1); #(shift_loc l 1) ◁ &uniq{α}ty]
             with "[] LFT HE Hna HL Hk"); last first.
     { rewrite tctx_interp_cons tctx_interp_singleton tctx_hasty_val tctx_hasty_val' //.
       iFrame. iApply (bor_shorten with "[] Hb"). iApply lft_incl_glb.
@@ -135,7 +135,7 @@ Section rwlockwriteguard_functions.
       apply cancel_local_update_empty, _. }
     iModIntro. wp_seq. iMod ("Hcloseα" with "Hβ") as "Hα".
     iMod ("Hclose" with "Hα HL") as "HL".
-    iApply (type_type _ _ _ [ x ◁ box (uninit 1)]%TC
+    iApply (type_type _ _ _ [ x ◁ box (uninit 1)]
             with "[] LFT HE Hna HL Hk"); first last.
     { rewrite tctx_interp_singleton tctx_hasty_val //. }
     iApply type_delete; [solve_typing..|].
