theories/typing/type_sum.v
@@ -132,7 +132,7 @@ Section case.
   Qed.
 
   Lemma type_case_shr E L C T p κ tyl el :
-    (p ◁ &shr{κ}sum tyl)%TC ∈ T →
+    p ◁ &shr{κ}sum tyl ∈ T →
     lctx_lft_alive E L κ →
     Forall2 (λ ty e, typed_body E L C ((p +ₗ #1 ◁ &shr{κ}ty) :: T) e) tyl el →
     typed_body E L C T (case: !p of el).
@@ -144,7 +144,7 @@ Section case.
   Lemma type_sum_assign_instr {E L} (i : nat) ty1 tyl ty ty2 p1 p2 :
     tyl !! i = Some ty →
     typed_write E L ty1 (sum tyl) ty2 →
-    typed_instruction E L [p1 ◁ ty1; p2 ◁ ty] (p1 <-{Σ i} p2) (λ _, [p1 ◁ ty2]%TC).
+    typed_instruction E L [p1 ◁ ty1; p2 ◁ ty] (p1 <-{Σ i} p2) (λ _, [p1 ◁ ty2]).
   Proof.
     iIntros (Hty Hw tid) "#LFT #HE $ HL Hp".
     rewrite tctx_interp_cons tctx_interp_singleton.
@@ -184,7 +184,7 @@ Section case.
   Lemma type_sum_unit_instr {E L} (i : nat) tyl ty1 ty2 p :
     tyl !! i = Some unit →
     typed_write E L ty1 (sum tyl) ty2 →
-    typed_instruction E L [p ◁ ty1] (p <-{Σ i} ()) (λ _, [p ◁ ty2]%TC).
+    typed_instruction E L [p ◁ ty1] (p <-{Σ i} ()) (λ _, [p ◁ ty2]).
   Proof.
     iIntros (Hty Hw tid) "#LFT #HE $ HL Hp". rewrite tctx_interp_singleton.
     wp_bind p. iApply (wp_hasty with "Hp"). iIntros (v Hv) "Hty".
@@ -215,7 +215,7 @@ Section case.
     typed_write E L ty1 (sum tyl) ty1' →
     typed_read E L ty2 ty ty2' →
     typed_instruction E L [p1 ◁ ty1; p2 ◁ ty2]
-               (p1 <-{ty.(ty_size),Σ i} !p2) (λ _, [p1 ◁ ty1'; p2 ◁ ty2']%TC).
+               (p1 <-{ty.(ty_size),Σ i} !p2) (λ _, [p1 ◁ ty1'; p2 ◁ ty2']).
   Proof.
     iIntros (Hty Hw Hr tid) "#LFT #HE Htl [HL1 HL2] Hp".
     rewrite tctx_interp_cons tctx_interp_singleton.
